concurrency/juicy/semax_safety_release.v
@@ -31,7 +31,6 @@ Require Import VST.veric.res_predicates.
 Require Import VST.veric.mem_lessdef.
 Require Import VST.veric.age_to_resource_at.
 Require Import VST.floyd.coqlib3.
-Require Import VST.sepcomp.semantics.
 Require Import VST.sepcomp.step_lemmas.
 Require Import VST.sepcomp.event_semantics.
 Require Import VST.sepcomp.semantics_lemmas.
@@ -99,7 +98,7 @@ Lemma safety_induction_release ge Gamma n state
 Proof.
   intros isrelease.
   intros I.
-  inversion I as [m tr sch_ tp Phi En envcoh compat sparse lock_coh safety wellformed unique E]. rewrite <-E in *.
+  inversion I as [m tr sch_ tp Phi En envcoh compat extcompat sparse lock_coh safety wellformed unique E]. rewrite <-E in *.
   unfold blocked_at_external in *.
   destruct isrelease as (i & cnti & sch & ci & args & -> & Eci & atex).
   pose proof (safety i cnti tt) as safei.
@@ -290,6 +289,10 @@ Proof.
 
   + (* env_coherence *)
     apply env_coherence_age_to. auto.
+
+  + (* external coherence *)
+    rewrite age_to_ghost_of.
+    destruct extcompat as [? J]; eapply ghost_fmap_join in J; eexists; eauto.
 
   + (* lock sparsity *)
     simpl.
