concurrency/juicy/semax_safety_spawn.v
@@ -33,7 +33,6 @@ Require Import VST.veric.mem_lessdef.
 Require Import VST.veric.age_to_resource_at.
 Require Import VST.veric.seplog.
 Require Import VST.floyd.coqlib3.
-Require Import VST.sepcomp.semantics.
 Require Import VST.sepcomp.step_lemmas.
 Require Import VST.sepcomp.event_semantics.
 Require Import VST.sepcomp.semantics_lemmas.
@@ -195,7 +194,7 @@ Lemma safety_induction_spawn ge Gamma n state
      state_invariant Jspec' Gamma (S n) state').
 Proof.
   intros isspawn I.
-  inversion I as [m tr sch_ tp Phi En envcoh compat sparse lock_coh safety wellformed unique E]. rewrite <-E in *.
+  inversion I as [m tr sch_ tp Phi En envcoh compat extcompat sparse lock_coh safety wellformed unique E]. rewrite <-E in *.
   unfold blocked_at_external in *.
   destruct isspawn as (i & cnti & sch & ci & args & -> & Eci & atex).
   pose proof (safety i cnti tt) as safei.
@@ -406,6 +405,9 @@ clear - Initcore.
 
   - (* env_coherence *)
     apply env_coherence_age_to; auto.
+
+  - rewrite age_to_ghost_of.
+    destruct extcompat as [? J]; eapply ghost_fmap_join in J; eexists; eauto.
 
   - (* lock sparsity *)
     apply lock_sparsity_age_to.
